\section*{Question 1: Part 1}

\paragraph{Given:}
\( f: \R^d \to \R \)
\begin{equation*}
    \func{f}{\x}
    =
    \half \qf{\x}{\Q}
    - \dotp{\b}{\x},
    \quad \Q \in \PD, \b \in \R^d
\end{equation*}

\( \Q \)-Gram-Schmidt recursion:
\begin{equation}
    \d_{k+1}
    =
    \p_{k+1}
    - \sum_{i = 0}^{k} \frac{\qf{\p_{k+1}}{\Q}[\d_i]}{\qf{\d_i}{\Q}} \d_i
\end{equation}

\subsection*{(a) \( \Q \)--conjugacy of \( \set{\d_k} \)}

Yes, the vectors produced by the above recursion are \( \Q \)--conjugate, which can be shown by induction.

\paragraph{Base case:}
\( k = 0 \)
\begin{align*}
    \implies
    \d_1
    & =
    \p_1
    - \frac{\qf{\p_1}{\Q}[\d_0]}{\qf{\d_0}{\Q}} \d_0
    \\
    \implies
    \qf{\d_1}{\Q}[\d_0]
    & =
    \qf{\p_1}{\Q}[\d_0]
    - \frac{\qf{\p_1}{\Q}[\d_0]}{\cancel{\qf{\d_0}{\Q}}} \cancel{\qf{\d_0}{\Q}}
    =
    \qf{\p_1}{\Q}[\d_0]
    - \qf{\p_1}{\Q}[\d_0]
    =
    0
\end{align*}

Thus, \( \d_1 \) is \( \Q \)--conjugate to \( \d_0 \), and the base case holds.

\paragraph{Inductive step:}
Assume that \( \d_i \) is \( \Q \)--conjugate to \( \d_j \) for all \( i, j \leq k \), \( i \neq j \).
We need to show that \( \d_{k+1} \) is \( \Q \)--conjugate to \( \d_j \) for all \( j \leq k \).

For \( j \leq k \), we  as follows
\begin{align*}
    \implies
    \qf{\d_{k+1}}{\Q}[\d_j]
    & =
    \qf{\p_{k+1}}{\Q}[\d_j]
    - \sum_{i = 0}^{k} \frac{\qf{\p_{k+1}}{\Q}[\d_i]}{\qf{\d_i}{\Q}} \qf{\d_i}{\Q}[\d_j]
    \\ & =
    \qf{\p_{k+1}}{\Q}[\d_j]
    - \frac{\qf{\p_{k+1}}{\Q}[\d_j]}{\cancel{\qf{\d_j}{\Q}}} \cancel{\qf{\d_j}{\Q}}
    - \sum_{\substack{i = 0 \\ i \neq j}}^{k} \frac{\qf{\p_{k+1}}{\Q}[\d_i]}{\qf{\d_i}{\Q}} \cancelto{0}{\qf{\d_i}{\Q}[\d_j]}
    \\ & =
    \qf{\p_{k+1}}{\Q}[\d_j]
    - \qf{\p_{k+1}}{\Q}[\d_j]
    - 0
    = 0
\end{align*}

Thus, \( \d_{k+1} \) is \( \Q \)--conjugate to \( \d_j \) for all \( j \leq k \), and the inductive step holds.

Hence, the vectors \( \set{\d_k} \) produced by the above recursion are \( \Q \)--conjugate.
